src/ssa/ssa_analysis.v
@@ -1,0 +1,823 @@
+Add LoadPath "./ott".
+Add LoadPath "./monads".
+Add LoadPath "./compcert".
+Add LoadPath "../../../theory/metatheory_8.3".
+Require Import ssa_def.
+Require Import ssa_lib.
+Require Import List.
+Require Import Arith.
+Require Import tactics.
+Require Import monad.
+Require Import trace.
+Require Import Metatheory.
+Require Import assoclist.
+Require Import Values.
+Require Import Memory.
+Require Import Integers.
+Require Import Coqlib.
+Require Import targetdata.
+Require Import Maps.
+Require Import Lattice.
+Require Import Iteration.
+Require Import Kildall.
+
+Export LLVMlib.
+
+(** * Domination analysis *)
+
+(** The type [Dominators] of compile-time approximations of domination. *)
+
+(** We equip this type of approximations with a semi-lattice structure.
+  The ordering is inclusion between the sets of values denoted by
+  the approximations. *)
+
+Module Dominators.
+  Section VarBoundSec.
+
+  Variable bound:atoms.
+
+  Record BoundedSet := mkBoundedSet {
+    bs_contents : atoms;
+    bs_bound : bs_contents [<=] bound
+  }.
+
+  Definition t := BoundedSet.
+
+  Definition eq (x y: t) :=
+    let '(mkBoundedSet cx _) := x in
+    let '(mkBoundedSet cy _) := y in
+    cx [=] cy.
+
+  Definition eq_refl: forall x, eq x x. 
+  Proof.
+    unfold eq. intro x. destruct x.
+    fsetdec.
+  Qed.
+
+  Definition eq_sym: forall x y, eq x y -> eq y x.
+  Proof.
+    unfold eq. intros x y J. destruct x. destruct y.
+    fsetdec.
+  Qed.
+  
+  Definition eq_trans: forall x y z, eq x y -> eq y z -> eq x z.
+  Proof.
+    unfold eq. intros x y z J1 J2. destruct x. destruct y. destruct z.
+    fsetdec.
+  Qed.
+
+  Lemma eq_dec: forall (x y: t), {eq x y} + {~ eq x y}.
+  Proof.
+    unfold eq. destruct x. destruct y.
+    apply AtomSetImpl.eq_dec.
+  Qed.
+
+  Definition beq (x y: t) := if eq_dec x y then true else false.
+
+  Lemma beq_correct: forall x y, beq x y = true -> eq x y.
+  Proof.
+    unfold beq; intros.  destruct (eq_dec x y). auto. congruence.
+  Qed.
+
+  Definition sub (x y: t) :=
+    let '(mkBoundedSet cx _) := x in
+    let '(mkBoundedSet cy _) := y in
+    cx [<=] cy.
+
+  Program Definition top : t := mkBoundedSet {} _.
+  Next Obligation.
+    fsetdec.
+  Qed.
+
+  Program Definition bot : t := mkBoundedSet bound _.
+  Next Obligation.
+    fsetdec.
+  Qed.
+
+  Definition ge (x y: t) : Prop := eq x top \/ eq y bot \/ sub x y.
+
+  Lemma ge_refl: forall x y, eq x y -> ge x y.
+  Proof.
+    unfold ge, eq, sub. destruct x, y. simpl.
+    intro J. right. right. fsetdec.
+  Qed.
+  Lemma ge_trans: forall x y z, ge x y -> ge y z -> ge x z.
+  Proof.
+    unfold ge, eq, sub. destruct x, y, z. simpl.
+    intros J1 J2.
+    destruct J1 as [J11 | [J12 | J13]]; try auto.
+      destruct J2 as [J21 | [J22 | J23]]; try auto.
+        assert (bound [=] empty) as EQ by fsetdec.
+        left. fsetdec.
+        right. left. fsetdec.
+      destruct J2 as [J21 | [J22 | J23]]; try auto.
+        left. fsetdec.
+        right. right. fsetdec.
+  Qed.
+  Lemma ge_compat: forall x x' y y', eq x x' -> eq y y' -> ge x y -> ge x' y'.
+  Proof.
+    unfold ge, eq, sub. destruct x, x', y, y'. simpl in *. 
+    intros J1 J2 J3.
+    destruct J3 as [J31 | [J32 | J33]].
+      left. fsetdec.
+      right. left. fsetdec.
+      right. right. fsetdec.
+  Qed.
+  Lemma ge_bot: forall x, ge x bot.
+  Proof.
+    unfold ge, eq, sub. destruct x. simpl. right. left. fsetdec.
+  Qed.
+  Lemma ge_top: forall x, ge top x.
+  Proof.
+    unfold ge, eq, sub. destruct x. simpl. left. fsetdec.
+  Qed.
+  Program Definition lub (x y: t) : t :=
+    let '(mkBoundedSet cx _) := x in
+    let '(mkBoundedSet cy _) := y in
+    mkBoundedSet (AtomSetImpl.inter cx cy) _.
+  Next Obligation.
+    fsetdec.
+  Qed.
+  Lemma lub_commut: forall x y, eq (lub x y) (lub y x).
+  Proof.
+    unfold lub, eq. destruct x, y. fsetdec.
+  Qed.
+  Lemma ge_lub_left: forall x y, ge (lub x y) x.
+  Proof.
+    unfold lub, ge, sub, eq. destruct x, y. simpl.
+    right. right. fsetdec.
+  Qed.
+
+  Program Definition add (x:t) (a:atom) : t := 
+    let '(mkBoundedSet cx _) := x in
+    if (AtomSetProperties.In_dec a bound) then
+      mkBoundedSet (AtomSetImpl.add a cx) _
+    else
+      x.
+  Next Obligation.
+  Admitted.
+
+  End VarBoundSec. 
+End Dominators.
+
+Module Dataflow_Solver_Var_Top (NS: NODE_SET).
+
+Module L := Dominators.
+
+Section Kildall.
+
+Variable bound : atoms.
+Definition dt := L.t bound.
+Variable successors: ATree.t (list atom).
+Variable transf: atom -> dt -> dt.
+Variable entrypoints: list (atom * dt).
+
+(** The state of the iteration has two components:
+- A mapping from program points to values of type [L.t] representing
+  the candidate solution found so far.
+- A worklist of program points that remain to be considered.
+*)
+
+Record state : Type :=
+  mkstate { st_in: AMap.t dt; st_wrk: NS.t }.
+
+(** Kildall's algorithm, in pseudo-code, is as follows:
+<<
+    while st_wrk is not empty, do
+        extract a node n from st_wrk
+        compute out = transf n st_in[n]
+        for each successor s of n:
+            compute in = lub st_in[s] out
+            if in <> st_in[s]:
+                st_in[s] := in
+                st_wrk := st_wrk union {s}
+            end if
+        end for
+    end while
+    return st_in
+>>
+
+The initial state is built as follows:
+- The initial mapping sets all program points to [L.bot], except
+  those mentioned in the [entrypoints] list, for which we take
+  the associated approximation as initial value.  Since a program
+  point can be mentioned several times in [entrypoints], with different
+  approximations, we actually take the l.u.b. of these approximations.
+- The initial worklist contains all the program points. *)
+
+Fixpoint start_state_in (ep: list (atom * dt)) : AMap.t dt :=
+  match ep with
+  | nil =>
+      AMap.init (L.bot _)
+  | (n, v) :: rem =>
+      let m := start_state_in rem in AMap.set n (L.lub _ m!!n v) m
+  end.
+
+Definition start_state :=
+  mkstate (start_state_in entrypoints) (NS.initial successors).
+
+(** [propagate_succ] corresponds, in the pseudocode,
+  to the body of the [for] loop iterating over all successors. *)
+
+Definition propagate_succ (s: state) (out: dt) (n: atom) :=
+  let oldl := s.(st_in)!!n in
+  let newl := L.lub _ oldl out in
+  if L.beq _ oldl newl
+  then s
+  else mkstate (AMap.set n newl s.(st_in)) (NS.add n s.(st_wrk)).
+
+(** [propagate_succ_list] corresponds, in the pseudocode,
+  to the [for] loop iterating over all successors. *)
+
+Fixpoint propagate_succ_list (s: state) (out: dt) (succs: list atom)
+                             {struct succs} : state :=
+  match succs with
+  | nil => s
+  | n :: rem => propagate_succ_list (propagate_succ s out n) out rem
+  end.
+
+(** [step] corresponds to the body of the outer [while] loop in the
+  pseudocode. *)
+
+Definition step (s: state) : AMap.t dt + state :=
+  match NS.pick s.(st_wrk) with
+  | None => 
+      inl _ s.(st_in)
+  | Some(n, rem) =>
+      inr _ (propagate_succ_list
+              (mkstate s.(st_in) rem)
+              (transf n s.(st_in)!!n)
+              (successors!!!n))
+  end.
+
+(** The whole fixpoint computation is the iteration of [step] from
+  the start state. *)
+
+Definition fixpoint : option (AMap.t dt) :=
+  PrimIter.iterate _ _ step start_state.
+
+(** ** Monotonicity properties *)
+
+(** We first show that the [st_in] part of the state evolves monotonically:
+  at each step, the values of the [st_in[n]] either remain the same or
+  increase with respect to the [L.ge] ordering. *)
+
+Definition in_incr (in1 in2: AMap.t dt) : Prop :=
+  forall n, L.ge _ in2!!n in1!!n.
+
+Lemma in_incr_refl:
+  forall in1, in_incr in1 in1.
+Proof.
+  unfold in_incr; intros. apply L.ge_refl. apply L.eq_refl.
+Qed.
+
+Lemma in_incr_trans:
+  forall in1 in2 in3, in_incr in1 in2 -> in_incr in2 in3 -> in_incr in1 in3.
+Proof.
+  unfold in_incr; intros. apply L.ge_trans with in2!!n; auto.
+Qed.
+
+Lemma propagate_succ_incr:
+  forall st out n,
+  in_incr st.(st_in) (propagate_succ st out n).(st_in).
+Proof.
+  unfold in_incr, propagate_succ; simpl; intros.
+  case (L.beq _ st.(st_in)!!n (L.lub _ st.(st_in)!!n out)).
+  apply L.ge_refl. apply L.eq_refl.
+  simpl. case (eq_atom_dec n n0); intro.
+  subst n0. rewrite AMap.gss. apply L.ge_lub_left.
+  rewrite AMap.gso; auto. apply L.ge_refl. apply L.eq_refl.
+Qed.
+
+Lemma propagate_succ_list_incr:
+  forall out scs st,
+  in_incr st.(st_in) (propagate_succ_list st out scs).(st_in).
+Proof.
+  induction scs; simpl; intros.
+  apply in_incr_refl.
+  apply in_incr_trans with (propagate_succ st out a).(st_in). 
+  apply propagate_succ_incr. auto.
+Qed. 
+
+Lemma fixpoint_incr:
+  forall res,
+  fixpoint = Some res -> in_incr (start_state_in entrypoints) res.
+Proof.
+  unfold fixpoint; intros.
+  change (start_state_in entrypoints) with start_state.(st_in).
+  eapply (PrimIter.iterate_prop _ _ step
+    (fun st => in_incr start_state.(st_in) st.(st_in))
+    (fun res => in_incr start_state.(st_in) res)).
+
+  intros st INCR. unfold step.
+  destruct (NS.pick st.(st_wrk)) as [ [n rem] | ].
+  apply in_incr_trans with st.(st_in). auto. 
+  change st.(st_in) with (mkstate st.(st_in) rem).(st_in). 
+  apply propagate_succ_list_incr. 
+  auto. 
+
+  eauto. apply in_incr_refl.
+Qed.
+
+(** ** Correctness invariant *)
+
+(** The following invariant is preserved at each iteration of Kildall's
+  algorithm: for all program points [n], either
+  [n] is in the worklist, or the inequations associated with [n]
+  ([st_in[s] >= transf n st_in[n]] for all successors [s] of [n])
+  hold.  In other terms, the worklist contains all nodes that do not
+  yet satisfy their inequations. *)
+
+Definition good_state (st: state) : Prop :=
+  forall n,
+  NS.In n st.(st_wrk) \/
+  (forall s, In s (successors!!!n) ->
+             L.ge _ st.(st_in)!!s (transf n st.(st_in)!!n)).
+
+(** We show that the start state satisfies the invariant, and that
+  the [step] function preserves it. *)
+
+Lemma start_state_good:
+  good_state start_state.
+Proof.
+  unfold good_state, start_state; intros.
+  case_eq (successors!n); intros.
+  left; simpl. eapply NS.initial_spec. eauto.
+  unfold successors_list. rewrite H. right; intros. contradiction.
+Qed.
+
+Lemma propagate_succ_charact:
+  forall st out n,
+  let st' := propagate_succ st out n in
+  L.ge _ st'.(st_in)!!n out /\
+  (forall s, n <> s -> st'.(st_in)!!s = st.(st_in)!!s).
+Proof.
+  unfold propagate_succ; intros; simpl.
+  predSpec (L.beq bound) (L.beq_correct bound)
+           ((st_in st) !! n) (L.lub _ (st_in st) !! n out).
+  split.
+  eapply L.ge_trans. apply L.ge_refl. apply H; auto.
+  eapply L.ge_compat. apply L.lub_commut. apply L.eq_refl. 
+  apply L.ge_lub_left. 
+  auto.
+
+  simpl. split.
+  rewrite AMap.gss.
+  eapply L.ge_compat. apply L.lub_commut. apply L.eq_refl. 
+  apply L.ge_lub_left. 
+  intros. rewrite AMap.gso; auto.
+Qed.
+
+Lemma propagate_succ_list_charact:
+  forall out scs st,
+  let st' := propagate_succ_list st out scs in
+  forall s,
+  (In s scs -> L.ge _ st'.(st_in)!!s out) /\
+  (~(In s scs) -> st'.(st_in)!!s = st.(st_in)!!s).
+Proof.
+  induction scs; simpl; intros.
+  tauto.
+  generalize (IHscs (propagate_succ st out a) s). intros [A B].
+  generalize (propagate_succ_charact st out a). intros [C D].
+  split; intros.
+  elim H; intro.
+  subst s.
+  apply L.ge_trans with (propagate_succ st out a).(st_in)!!a.
+  apply propagate_succ_list_incr. assumption.
+  apply A. auto.
+  transitivity (propagate_succ st out a).(st_in)!!s.
+  apply B. tauto.
+  apply D. tauto.
+Qed.
+
+Lemma propagate_succ_incr_worklist:
+  forall st out n x,
+  NS.In x st.(st_wrk) -> NS.In x (propagate_succ st out n).(st_wrk).
+Proof.
+  intros. unfold propagate_succ. 
+  case (L.beq _ (st_in st) !! n (L.lub _ (st_in st) !! n out)).
+  auto.
+  simpl. rewrite NS.add_spec. auto.
+Qed.
+
+Lemma propagate_succ_list_incr_worklist:
+  forall out scs st x,
+  NS.In x st.(st_wrk) -> NS.In x (propagate_succ_list st out scs).(st_wrk).
+Proof.
+  induction scs; simpl; intros.
+  auto.
+  apply IHscs. apply propagate_succ_incr_worklist. auto.
+Qed.
+
+Lemma propagate_succ_records_changes:
+  forall st out n s,
+  let st' := propagate_succ st out n in
+  NS.In s st'.(st_wrk) \/ st'.(st_in)!!s = st.(st_in)!!s.
+Proof.
+  simpl. intros. unfold propagate_succ. 
+  case (L.beq _ (st_in st) !! n (L.lub _ (st_in st) !! n out)).
+  right; auto.
+  case (eq_atom_dec s n); intro.
+  subst s. left. simpl. rewrite NS.add_spec. auto.
+  right. simpl. apply AMap.gso. auto.
+Qed.
+
+Lemma propagate_succ_list_records_changes:
+  forall out scs st s,
+  let st' := propagate_succ_list st out scs in
+  NS.In s st'.(st_wrk) \/ st'.(st_in)!!s = st.(st_in)!!s.
+Proof.
+  induction scs; simpl; intros.
+  right; auto.
+  elim (propagate_succ_records_changes st out a s); intro.
+  left. apply propagate_succ_list_incr_worklist. auto.
+  rewrite <- H. auto.
+Qed.
+
+Lemma step_state_good:
+  forall st n rem,
+  NS.pick st.(st_wrk) = Some(n, rem) ->
+  good_state st ->
+  good_state (propagate_succ_list (mkstate st.(st_in) rem)
+                                  (transf n st.(st_in)!!n)
+                                  (successors!!!n)).
+Proof.
+  unfold good_state. intros st n rem WKL GOOD x.
+  generalize (NS.pick_some _ _ _ WKL); intro PICK.
+  set (out := transf n st.(st_in)!!n).
+  elim (propagate_succ_list_records_changes 
+          out (successors!!!n) (mkstate st.(st_in) rem) x).
+  intro; left; auto.
+  simpl; intros EQ. rewrite EQ.
+  (* Case 1: x = n *)
+  case (eq_atom_dec x n); intro.
+  subst x.
+  right; intros.
+  elim (propagate_succ_list_charact out (successors!!!n)
+          (mkstate st.(st_in) rem) s); intros.
+  auto.
+  (* Case 2: x <> n *)
+  elim (GOOD x); intro.
+  (* Case 2.1: x was already in worklist, still is *)
+  left. apply propagate_succ_list_incr_worklist.
+  simpl. rewrite PICK in H. elim H; intro. congruence. auto.
+  (* Case 2.2: x was not in worklist *)
+  right; intros.
+  case (In_dec eq_atom_dec s (successors!!!n)); intro.
+  (* Case 2.2.1: s is a successor of n, it may have increased *)
+  apply L.ge_trans with st.(st_in)!!s.
+  change st.(st_in)!!s with (mkstate st.(st_in) rem).(st_in)!!s.
+  apply propagate_succ_list_incr. 
+  auto.
+  (* Case 2.2.2: s is not a successor of n, it did not change *)
+  elim (propagate_succ_list_charact out (successors!!!n)
+          (mkstate st.(st_in) rem) s); intros.
+  rewrite H2. simpl. auto. auto.
+Qed.
+
+(** ** Correctness of the solution returned by [iterate]. *)
+
+(** As a consequence of the [good_state] invariant, the result of
+  [fixpoint], if defined, is a solution of the dataflow inequations,
+  since [st_wrk] is empty when the iteration terminates. *)
+
+Theorem fixpoint_solution:
+  forall res n s,
+  fixpoint = Some res ->
+  In s (successors!!!n) ->
+  L.ge _ res!!s (transf n res!!n).
+Proof.
+  assert (forall res, fixpoint = Some res ->
+          forall n s,
+          In s successors!!!n ->
+          L.ge _ res!!s (transf n res!!n)).
+  unfold fixpoint. intros res PI. pattern res. 
+  eapply (PrimIter.iterate_prop _ _ step good_state).
+
+  intros st GOOD. unfold step. 
+  caseEq (NS.pick st.(st_wrk)). 
+  intros [n rem] PICK. apply step_state_good; auto. 
+  intros. 
+  elim (GOOD n); intro. 
+  elim (NS.pick_none _ n H). auto.
+  auto.
+
+  eauto. apply start_state_good. eauto.
+Qed.
+
+(** As a consequence of the monotonicity property, the result of
+  [fixpoint], if defined, is pointwise greater than or equal the
+  initial mapping.  Therefore, it satisfies the additional constraints
+  stated in [entrypoints]. *)
+
+Lemma start_state_in_entry:
+  forall ep n v,
+  In (n, v) ep ->
+  L.ge _ (start_state_in ep)!!n v.
+Proof.
+  induction ep; simpl; intros.
+  elim H.
+  elim H; intros.
+  subst a. rewrite AMap.gss.
+  eapply L.ge_compat. apply L.lub_commut. apply L.eq_refl. 
+  apply L.ge_lub_left.
+  destruct a. rewrite AMap.gsspec. case (eq_atom_dec n a); intro.
+  subst a. apply L.ge_trans with (start_state_in ep)!!n.
+  apply L.ge_lub_left. auto.
+  auto.
+Qed.
+
+Theorem fixpoint_entry:
+  forall res n v,
+  fixpoint = Some res ->
+  In (n, v) entrypoints ->
+  L.ge _ res!!n v.
+Proof.
+  intros.
+  apply L.ge_trans with (start_state_in entrypoints)!!n.
+  apply fixpoint_incr. auto.
+  apply start_state_in_entry. auto.
+Qed.
+
+(** ** Preservation of a property over solutions *)
+
+Variable P: dt -> Prop.
+Hypothesis P_bot: P (L.bot _).
+Hypothesis P_lub: forall x y, P x -> P y -> P (L.lub _ x y).
+Hypothesis P_transf: forall pc x, P x -> P (transf pc x).
+Hypothesis P_entrypoints: forall n v, In (n, v) entrypoints -> P v.
+
+Theorem fixpoint_invariant:
+  forall res pc,
+  fixpoint = Some res ->
+  P res!!pc.
+Proof.
+  assert (forall ep,
+          (forall n v, In (n, v) ep -> P v) ->
+          forall pc, P (start_state_in ep)!!pc).
+    induction ep; intros; simpl.
+    rewrite AMap.gi. auto.
+    simpl in H.
+    assert (P (start_state_in ep)!!pc). apply IHep. eauto.  
+    destruct a as [n v]. rewrite AMap.gsspec. destruct (eq_atom_dec pc n).
+    apply P_lub. subst. auto. eapply H. left; reflexivity. auto.
+  set (inv := fun st => forall pc, P (st.(st_in)!!pc)).
+  assert (forall st v n, inv st -> P v -> inv (propagate_succ st v n)).
+    unfold inv, propagate_succ. intros. 
+    destruct (L.beq _ (st_in st)!!n (L.lub _ (st_in st)!!n v)).
+    auto. simpl. rewrite AMap.gsspec. destruct (eq_atom_dec pc n). 
+    apply P_lub. subst n; auto. auto.
+    auto.
+  assert (forall l0 st v, inv st -> P v -> inv (propagate_succ_list st v l0)).
+    induction l0; intros; simpl. auto.
+    apply IHl0; auto.
+  assert (forall res, fixpoint = Some res -> forall pc, P res!!pc).
+    unfold fixpoint. intros res0 RES0. pattern res0.
+    eapply (PrimIter.iterate_prop _ _ step inv).
+    intros. unfold step. destruct (NS.pick (st_wrk a)) as [[n rem] | ].
+    apply H1. auto. apply P_transf. apply H2.
+    assumption.
+    eauto. 
+    unfold inv, start_state; simpl. auto. 
+  intros. auto.
+Qed.
+
+End Kildall.
+
+End Dataflow_Solver_Var_Top.
+
+Definition successors_terminator (tmn: terminator) : ls :=
+match tmn with
+| insn_return _ _ _ => nil
+| insn_return_void _ => nil
+| insn_br _ _ l1 l2 => l1::l2::nil
+| insn_br_uncond _ l1 => l1::nil
+| insn_unreachable _ => nil
+end.
+
+Fixpoint successors_blocks (bs: blocks) : ATree.t ls :=
+match bs with
+| nil => ATree.empty ls
+| block_intro l0 _ _ tmn :: bs' => 
+    ATree.set l0 (successors_terminator tmn) (successors_blocks bs')
+end.
+
+Fixpoint successors (f: fdef) : ATree.t ls :=
+let '(fdef_intro _ bs) := f in
+successors_blocks bs.
+
+Definition transfer (bound: atoms) (lbl: l) (before: Dominators.t bound) :=
+  Dominators.add _ before lbl.
+
+(** The static analysis itself is then an instantiation of Kildall's
+  generic solver for forward dataflow inequations. [analyze f]
+  returns a mapping from program points to mappings of pseudo-registers
+  to approximations.  It can fail to reach a fixpoint in a reasonable
+  number of iterations, in which case [None] is returned. *)
+
+Module DomDS := Dataflow_Solver_Var_Top(AtomNodeSet).
+
+Fixpoint bound_blocks (bs: blocks) :  atoms :=
+match bs with
+| nil => {}
+| block_intro l0 _ _ tmn :: bs' => {{l0}} `union` (bound_blocks bs')
+end.
+
+Fixpoint bound_fdef (f: fdef) :  atoms :=
+let '(fdef_intro _ bs) := f in
+bound_blocks bs.
+
+Program Definition dom_analyze (f: fdef): AMap.t (Dominators.t (bound_fdef f)) :=
+  let bound := bound_fdef f in
+  let top := Dominators.top bound in
+  match getEntryBlock f with
+  | Some (block_intro le _ _ _) =>
+      match DomDS.fixpoint bound (successors f) (transfer bound) 
+        ((le, Dominators.mkBoundedSet _ {{le}} _) :: nil) with
+      | None => AMap.init top
+      | Some res => res
+      end
+  | None => AMap.init top
+  end.
+Next Obligation.
+  destruct f. 
+  destruct b; simpl in *; inv Heq_anonymous. 
+    fsetdec.
+Qed.
+
+Definition blockDominates (f: fdef) (b1 b2: block) : Prop :=
+let '(block_intro l1 _ _ _) := b1 in
+let '(block_intro l2 _ _ _) := b2 in
+let 'dt := dom_analyze f in
+let '(Dominators.mkBoundedSet els _) := AMap.get l2 dt in
+AtomSetProperties.In_dec l1 els.
+
+Definition blockDominatesB (f: fdef) (b1 b2: block) : Prop :=
+let '(block_intro l1 _ _ _) := b1 in
+let '(block_intro l2 _ _ _) := b2 in
+let 'dt := dom_analyze f in
+let '(Dominators.mkBoundedSet els _) := AMap.get l2 dt in
+if AtomSetProperties.In_dec l1 els then true else false.
+
+Definition insnDominates (i1 i2:insn) (b:block) : Prop :=
+match b with 
+| (block_intro l5 ps cs tmn) =>
+    match (i1, i2) with
+    | (insn_cmd _, insn_terminator _) => True  
+    | (insn_phinode _, insn_terminator _) => True
+    | (insn_phinode _, insn_cmd _) => True
+    | (insn_cmd c1, insn_cmd c2) => 
+      (exists cs1, exists cs2, exists cs3, cs = cs1++(c1::cs2)++(c2::cs3))
+    | (insn_phinode p1, insn_phinode p2) => 
+      (exists ps1, exists ps2, exists ps3, ps = ps1++(p1::ps2)++(p2::ps3))
+    | _ => False
+    end
+end.
+
+Module ReachDS := Dataflow_Solver(LBoolean)(AtomNodeSet).
+
+Definition reachable_aux (f: fdef) : option (AMap.t bool) :=
+  match getEntryBlock f with
+  | Some (block_intro le _ _ _) =>
+     ReachDS.fixpoint (successors f) (fun pc r => r) ((le, true) :: nil)
+  | None => None
+  end.
+
+Definition reachable (f: fdef) : AMap.t bool :=
+  match reachable_aux f with  
+  | None => AMap.init true
+  | Some rs => rs
+  end.
+
+Definition isReachableFromEntry (f:fdef) (b1:block) : Prop :=
+let '(block_intro l1 _ _ _) := b1 in
+AMap.get l1 (reachable f).
+ 
+(* blocks to CFG, which may not be useful. *)
+(*
+Fixpoint blocks_to_Vset (bs:blocks) : V_set :=
+match bs with
+| nil => V_empty
+| block_intro l _ _ _ :: bs' => V_union (V_single (index l)) (blocks_to_Vset bs')
+end.
+
+Fixpoint blocks_to_Aset (bs:blocks) : A_set :=
+match bs with
+| nil => A_empty
+| block_intro l0 _ _ (insn_br _ _ l1 l2) :: bs' => 
+    A_union (A_single (A_ends (index l0) (index l1)))
+      (A_union (A_single (A_ends (index l0) (index l2))) (blocks_to_Aset bs'))
+| block_intro l0 _ _ (insn_br_uncond _ l1) :: bs' => 
+    A_union (A_single (A_ends (index l0) (index l1))) (blocks_to_Aset bs')
+| block_intro l0 _ _ _ :: bs' => blocks_to_Aset bs'
+end.
+
+Lemma blocks_to_Vset_spec : forall (blocks5 : blocks) (l0 : l) 
+  (H4 : l0 `notin` dom (genLabel2Block_blocks blocks5)),
+  ~ blocks_to_Vset blocks5 (index l0).
+Proof.
+  intros.
+  induction blocks5; intro J.
+    inversion J.
+
+    destruct a. simpl in *.
+    inversion J; subst.
+      inversion H; subst.
+      fsetdec.
+
+      apply IHblocks5; try solve [auto | fsetdec].
+Qed.
+
+Lemma blocks_to_CFG_add_Vs : forall F bs,
+  cfg_blocks F bs ->
+  uniq (genLabel2Block_blocks bs) ->
+  exists cfg : Digraph (blocks_to_Vset bs) A_empty, True.
+Proof.
+  intros F bs Hwfbs Huniq. 
+  induction Hwfbs; simpl; intros.
+    exists D_empty. auto.
+    
+    destruct block5 as [l0 ? ? tmn].
+    inversion Huniq; subst.
+    apply IHHwfbs in H2.
+    destruct H2 as [cfg _].
+    assert (~ blocks_to_Vset blocks5 (index l0)) as J.
+      eapply blocks_to_Vset_spec; eauto.
+    destruct tmn;
+      apply D_vertex with (x:=index l0) in cfg; 
+        try solve [auto | exists cfg; auto].
+Qed.
+
+Lemma Included_union_right : forall U (E F C: U_set U), 
+  Included U (Union U E F) C ->
+  Included U F C.
+Proof.
+        unfold Included in |- *; intros.
+        apply H. apply In_right. trivial.
+Qed.
+
+Lemma Included_union_left : forall U (E F C: U_set U), 
+  Included U (Union U E F) C ->
+  Included U E C.
+Proof.
+        unfold Included in |- *; intros.
+        apply H. apply In_left. trivial.
+Qed.
+
+Lemma blocks_to_CFG_add_As : forall F bs Vs,
+  cfg_blocks F bs ->
+  uniq (genLabel2Block_blocks bs) ->
+  V_included (blocks_to_Vset bs) Vs ->
+  Digraph Vs A_empty ->
+  exists cfg : Digraph Vs (blocks_to_Aset bs), True.
+Proof.
+  intros F bs Vs Hwfbs Huniq Hinc Hcfg. 
+  induction Hwfbs; simpl in *; intros.
+    exists Hcfg. auto.
+    
+    destruct block5 as [l0 ? ? tmn]; simpl in *.
+    inversion Huniq; subst.
+    assert (J:=Hinc).
+    apply Included_union_left in J.
+    apply Included_union_right in Hinc.
+    apply IHHwfbs in H2; auto.
+    destruct H2 as [cfg _].
+    destruct tmn.
+      exists cfg. auto.
+      exists cfg. auto.
+
+      apply D_arc with (x:=index l0)(y:=index l2) in cfg.
+        apply D_arc with (x:=index l0)(y:=index l1) in cfg.
+          exists cfg. auto.
+          unfold Included in J. apply J. unfold V_single. apply In_single.
+         
+          admit.
+          admit.
+          admit.
+          admit.
+          admit.
+      admit.
+      exists cfg. auto.
+Qed.
+
+Lemma blocks_to_CFG : forall F bs,
+  cfg_blocks F bs ->
+  uniq (genLabel2Block_blocks bs) ->
+  exists cfg : Digraph (blocks_to_Vset bs) (blocks_to_Aset bs), True.
+Proof.
+  intros F bs Hwfbs Huniq.
+  assert (J:=Hwfbs).
+  apply blocks_to_CFG_add_Vs in J; auto.
+  destruct J as [cfg _].
+  eapply blocks_to_CFG_add_As; eauto.
+    unfold V_included, Included. auto.
+Qed.
+*)
+
+(*****************************)
+(*
+*** Local Variables: ***
+*** coq-prog-name: "coqtop" ***
+*** coq-prog-args: ("-emacs-U" "-I" "~/SVN/sol/vol/src/ssa/monads" "-I" "~/SVN/sol/vol/src/ssa/ott" "-I" "~/SVN/sol/vol/src/ssa/compcert" "-I" "~/SVN/sol/theory/metatheory_8.3" "-I" "~/SVN/sol/vol/src/TV") ***
+*** End: ***
+ *)
